\documentclass[10pt,a4paper]{article}
\usepackage[latin1]{inputenc}
\usepackage{amsmath}
\usepackage{amsfonts}
\usepackage{amssymb}
\usepackage{graphicx}
\usepackage{lmodern}
\usepackage{hyperref}
\usepackage{cleveref}
\author{Daniel Celis Garza}
\title{Interpolation Notes}
\date{\today}
\begin{document}
\maketitle
\section{Neville's Algorithm}
For $n = 4$
\begin{align*}
x_{1}:\qquad& y_{1} =& P_{1,1} 	&					\hspace{-2cm}&				   \\
			&		 & 	& P_{1,2}			\hspace{-2cm}&				   \\
x_{2}:\qquad& y_{2} =& P_{2,2} 	&\qquad P_{1,2,3}	\hspace{-2cm}&				   \\
			&		 &		 	& P_{2,3}			\hspace{-2cm}& P_{1,2,3,4}	   \\
x_{3}:\qquad& y_{3}	=& P_{3,3}	&\qquad P_{2,3,4}	\hspace{-2cm}&				   \\
			&		 & 	& P_{3,4}			\hspace{-2cm}&				   \\
x_{1}:\qquad& y_{4} =& P_{4,4} 	&					\hspace{-2cm}&				   \\
\end{align*}

\begin{subequations}\label{e:nev}
\begin{align}
& P_{i,i} = y_{i}~, && 0\le i \le n \\
& P_{i,j} =
\dfrac{
(x_j-x)P_{i,j-1} + (x-x_i)P_{i+1,j}
}
{
x_{j}-x_{i}
}~, && 0\le i < j \le n
\end{align}
\end{subequations}

The original formula is:

\begin{align}\label{e:lag}
^{n}P(x) = \sum\limits_{i=0}^{n}\left(
\prod\limits_{\substack{0 \le j \le n \\ j \ne i}}
\dfrac{x-x_{j}}{x_{i}-x_{j}}
\right)y_{i}
\end{align}

For $n = 2$ \cref{e:nev} is
\begin{align*}
P_{1,2} &= \dfrac{(x_{2} - x)P_{1,1} + (x-x_{1})P_{2,2}}{x_{2}-x_{1}}\\
P_{1,2} &= \dfrac{(x_{2} - x)y_{1} + (x-x_{1})y_{2}}{x_{2}-x_{1}}	 \\
\end{align*}
and \cref{e:lag} is
\begin{align*}
^{n}P &= \dfrac{x-x_{2}}{x_{1}-x_{2}}y_{1} + \dfrac{x-x_{1}}{x_{2}-x_{1}}y_{2} \\
^{n}P &= \dfrac{-(x_{2}-x)}{-(x_{2}-x_{1})}y_{1} + \dfrac{x-x_{1}}{x_{2}-x_{1}}y_{2} \\
\end{align*}
\end{document}